[prev_node] and [next_node] return nullable nodes. See msg.
By making this change, we no longer _require_ the paradigm of "check
before movement", but instead allow for both "check before movement"
and "check after movement". Since the second one is more idiomatic in
C, this leads to cleaner code.

ind/DoublyLinkedListIface.fst
@@ -573,13 +573,19 @@ let has_prev d n =
 let next_node d n =
   let h0 = HST.get () in
   lemma_node_in_valid_dll_is_valid h0 d n;
-  DLL.extract_nodelist_conn h0 (as_list h0 d) (L.index_of (as_list h0 d) n);
+  if L.index_of (as_list h0 d) n < L.length (as_list h0 d) - 1 then (
+    DLL.extract_nodelist_conn h0 (as_list h0 d) (L.index_of (as_list h0 d) n)
+  ) else (
+    L.lemma_unsnoc_is_last (as_list h0 d)
+  );
   (!*n).DLL.flink
 
 let prev_node d n =
   let h0 = HST.get () in
   lemma_node_in_valid_dll_is_valid h0 d n;
-  DLL.extract_nodelist_conn h0 (as_list h0 d) (L.index_of (as_list h0 d) n - 1);
+  if L.index_of (as_list h0 d) n > 0 then (
+    DLL.extract_nodelist_conn h0 (as_list h0 d) (L.index_of (as_list h0 d) n - 1)
+  ) else ();
   (!*n).DLL.blink
 
 /// Stateful DoublyLinkedList operations
